Change possibilities to use state instead of traces

Core/Logic.v
@@ -7,39 +7,72 @@ From Coq Require Import
   Lists.List
   Init.Nat
   Logic.FunctionalExtensionality
-  Logic.PropExtensionality.
+  Logic.PropExtensionality
+  Relations.Relation_Operators.
 
-Definition Prec E VE F :=
+Record Poss {F} {VF : Spec F} := MkPoss {
+  PState : VF.(State);
+  PCalls : ThreadName -> option {A : Type & F A};
+  PRets : ThreadName -> option {A : Type & A}
+}.
+Arguments Poss {F} VF.
+
+Definition Prec {E F} (VE : Spec E) (VF : Spec F) :=
   @InterState E F VE ->
-  Trace (ThreadEvent F) ->
+  Poss VF ->
   Prop.
 
-Definition Relt E VE F :=
-  @InterState E F VE -> Trace (ThreadEvent F) ->
-  @InterState E F VE -> Trace (ThreadEvent F) ->
+Definition Relt {E F} (VE : Spec E) (VF : Spec F) :=
+  @InterState E F VE ->
+  Poss VF ->
+  @InterState E F VE ->
+  Poss VF ->
   Prop.
 
-Definition Post E VE F A :=
-  A -> Relt E VE F.
+Definition Post {E F} (VE : Spec E) (VF : Spec F) A :=
+  A -> Relt VE VF.
 
-Inductive RTC {E VE F} {R : Relt E VE F} : Relt E VE F :=
-| RTCRefl s ρ : RTC s ρ s ρ
-| RTCTrans s ρ t σ r τ :
+Definition StRelt {E} (VE : Spec E) F :=
+  @InterState E F VE ->
+  @InterState E F VE ->
+  Prop.
+
+Inductive RTC {E F} {VE : Spec E} {VF : Spec F} (R : Relt VE VF) : Relt VE VF :=
+| RTCRefl s ρ : RTC R s ρ s ρ
+| RTCStep s ρ t σ r τ :
     R s ρ t σ ->
-    RTC t σ r τ ->
-    RTC s ρ r τ.
-Arguments RTC {E VE F} R.
+    RTC R t σ r τ ->
+    RTC R s ρ r τ.
 
-Definition ReltToPrec {E VE F} (R : Relt E VE F) : Prec E VE F :=
+Definition prComp {E F} {VE : Spec E} {VF : Spec F} (P : Prec VE VF) (R : Relt VE VF) : Relt VE VF :=
+  fun s ρ t σ => P s ρ /\ R s ρ t σ.
+
+Definition ReltToPrec {E F} {VE : Spec E} {VF : Spec F} (R : Relt VE VF) : Prec VE VF :=
   fun t σ => exists s ρ, R s ρ t σ.
 Coercion ReltToPrec : Relt >-> Prec.
 
-Definition PrecCompose {E VE F} (P : Prec E VE F) (R : Relt E VE F) : Prec E VE F :=
+Definition PrecToRelt {E F} {VE : Spec E} {VF : Spec F} (P : Prec VE VF) : Relt VE VF :=
+  fun s ρ t σ =>
+    P s ρ /\
+    s = t /\
+    ρ = σ.
+
+Definition PostToRelt {E F} {VE : Spec E} {VF : Spec F} {A} (Q : Post VE VF A) : Relt VE VF :=
+  fun s ρ t σ => exists v, Q v s ρ t σ.
+Coercion PostToRelt : Post >-> Relt.
+
+Definition StReltToRelt {E F} {VE : Spec E} {VF : Spec F} (Q : StRelt VE F) : Relt VE VF :=
+  fun s ρ t σ =>
+    Q s t /\
+    ρ = σ.
+Coercion StReltToRelt : StRelt >-> Relt.
+
+Definition PrecCompose {E F} {VE : Spec E} {VF : Spec F} (P : Prec VE VF) (R : Relt VE VF) : Prec VE VF :=
   fun t σ => exists s ρ, P s ρ /\ R s ρ t σ.
 
 Notation "R <<- G" := (PrecCompose R G) (left associativity, at level 37).
 
-Definition ReltCompose {E VE F} (R G : Relt E VE F) : Relt E VE F :=
+Definition ReltCompose {E F} {VE : Spec E} {VF : Spec F} (R G : Relt VE VF) : Relt VE VF :=
   fun s ρ r τ => exists t σ, R s ρ t σ /\ G t σ r τ.
 Notation "R ->> G" := (ReltCompose R G) (right associativity, at level 39).
 
@@ -47,135 +80,159 @@ Class HasSub A :=
   sub : A -> A -> Prop.
 Notation "P ==> Q" := (sub P Q) (right associativity, at level 41).
 
-Global Instance subPrec E VE F : HasSub (@Prec E VE F) :=
+Global Instance subPrec {E F} {VE : Spec E} {VF : Spec F} : HasSub (Prec VE VF) :=
   fun P Q => forall s ρ, P s ρ -> Q s ρ.
 
-Global Instance subRelt E VE F : HasSub (Relt E VE F) :=
+Global Instance subRelt {E F} {VE : Spec E} {VF : Spec F} : HasSub (Relt VE VF) :=
   fun P Q => forall s ρ t σ, P s ρ t σ -> Q s ρ t σ.
 
-Class HasStable {E VE F} A :=
-  Stable : Relt E VE F -> A -> Prop.
+Class HasStable {E F} {VE : Spec E} {VF : Spec F} A :=
+  Stable : Relt VE VF -> A -> Prop.
 
-Global Instance stableRelt {E VE F} : HasStable (Relt E VE F) :=
+Global Instance stableRelt {E F} {VE : Spec E} {VF : Spec F} : HasStable (Relt VE VF) :=
   fun R Q => (R ->> Q ==> Q) /\ (Q ->> R ==> Q).
 
-Global Instance stablePrec {E VE F} : HasStable (@Prec E VE F) :=
+Global Instance stablePrec {E F} {VE : Spec E} {VF : Spec F} : HasStable (Prec VE VF) :=
   fun R P => P <<- R ==> P.
 
-Global Instance stablePost {E VE F A} : HasStable (Post E VE F A) :=
+Global Instance stablePost {E F} {VE : Spec E} {VF : Spec F} {A} : HasStable (Post VE VF A) :=
   fun R Q => forall v, stableRelt R (Q v).
 
-Definition id {E VE F} : Relt E VE F :=
+Definition id {E F VE VF} : @Relt E F VE VF :=
   fun s ρ t σ => s = t /\ ρ = σ.
 
-Definition ptop {E VE F} : @Prec E VE F :=
+Definition ptop {E F VE VF} : @Prec E F VE VF :=
   fun _ _ => True.
-Definition rtop {E VE F} : Relt E VE F :=
+Definition rtop {E F VE VF} : @Relt E F VE VF :=
   fun _ _ _ _ => True.
 
-Notation "ρ --> σ" := (exists t, AllRetEv t /\ LinRw (ρ ++ t) σ)
-  (at level 20).
+Variant PossStep {F} {VF : Spec F} : Poss VF -> Poss VF -> Prop :=
+| PInvoke i ρ σ A (m : F A) :
+  σ.(PState) = ρ.(PState) ->
+  σ.(PCalls) = updThs ρ.(PCalls) i (Some (existT _ A m)) ->
+  σ.(PRets) = ρ.(PRets) ->
+  PossStep ρ σ
+| PCommitCall i ρ σ A (m : F A) :
+  VF.(Step) ρ.(PState) (i, CallEv m) σ.(PState) ->
+  updThs σ.(PCalls) i (Some (existT _ A m)) = ρ.(PCalls) ->
+  σ.(PRets) = ρ.(PRets) ->
+  PossStep ρ σ
+| PCommitRet i ρ σ A (m : F A) v :
+  VF.(Step) ρ.(PState) (i, RetEv m v) σ.(PState) ->
+  σ.(PCalls) = ρ.(PCalls) ->
+  σ.(PRets) = updThs ρ.(PRets) i (Some (existT _ A v)) ->
+  PossStep ρ σ
+| PReturn i ρ σ A v :
+  σ.(PState) = ρ.(PState) ->
+  σ.(PCalls) = ρ.(PCalls) ->
+  updThs σ.(PRets) i (Some (existT _ A v)) = ρ.(PRets) ->
+  PossStep ρ σ.
 
-Definition Commit {E VE F} VF i (impl : Impl E F)
-  (G : Relt E VE F)
-  (P : @Prec E VE F)
+Definition Commit {E F} {VE : Spec E} {VF : Spec F} i (impl : Impl E F)
+  (G : Relt VE VF)
+  (P : Prec VE VF)
   (ev : @Event E)
-  (Q : Relt E VE F) :=
+  (Q : Relt VE VF) :=
   forall s ρ t,
-  LinToSpec ρ VF ->
   P s ρ ->
   InterStep (impl:=impl) i s (i, liftUEv ev) t ->
     exists σ,
+      clos_refl_trans _ PossStep ρ σ /\
       Q s ρ t σ /\
-      G s ρ t σ /\
-      ρ --> σ.
+      G s ρ t σ.
 
-CoInductive VerifyProg {E VE F} VF i (impl : Impl E F) : Relt E VE F -> Relt E VE F -> forall (A: Type), @Prec E VE F -> Prog E A -> Post E VE F A -> Prop :=
-| SafeReturn A v R G P Q :
-    (forall s ρ t σ, P s ρ -> Q v s ρ t σ) ->
-    VerifyProg VF i impl R G A P (Return v) Q
-| SafeBind A B R G P QI QR S (m : E A) (k : A -> Prog E B) :
-    Stable R QI ->
-    Stable R QR ->
-    Commit VF i impl G P (CallEv m) QI ->
-    (forall v,
-      Commit VF i impl G QI (RetEv m v) (QR v) /\
-      VerifyProg VF i impl R G B (QR v) (k v) S) ->
-    VerifyProg VF i impl R G B P (Bind m k) S
-| SafeNoOp A R G P C Q :
-    VerifyProg VF i impl R G A P C Q ->
-    VerifyProg VF i impl R G A P (NoOp C) Q
+CoInductive SafeProg {E F} {VE : Spec E} {VF : Spec F} i (impl : Impl E F) : Relt VE VF -> Relt VE VF -> forall (A : Type), Relt VE VF -> Prog E A -> Post VE VF A -> Prop :=
+| SafeReturn A v R G Q Q0 :
+  Q ==> Q0 v ->
+  SafeProg i impl R G A Q (Return v) Q0
+| SafeBind A B R G (Q : Relt VE VF) QI QR Q0 (m : E A) k :
+  Stable R QI ->
+  Stable R QR ->
+  Commit i impl G Q (CallEv m) QI ->
+  (forall v,
+    Commit i impl G (Q ->> QI) (RetEv m v) (QR v) /\
+    SafeProg i impl R G B (Q ->> QI ->> QR v) (k v) Q0) ->
+  SafeProg i impl R G B Q (Bind m k) Q0
+| SafeNoOp R G A Q C Q0 :
+  SafeProg i impl R G A Q C Q0 ->
+  SafeProg i impl R G A Q (NoOp C) Q0
 .
-Arguments VerifyProg {E VE F} VF i impl R G {A} P C Q.
-  
-Inductive TraceIdle i {F} : Trace (ThreadEvent F) -> Prop :=
-| NilIdle : TraceIdle i nil
-| SkipIdle {j e ρ} :
-    i <> j ->
-    TraceIdle i ρ ->
-    TraceIdle i (cons (j, e) ρ)
-| ConsIdle {A m v ρ} :
-    TraceIdle i ρ ->
-    TraceIdle i (cons (i, CallEv m) (cons (i, RetEv (Ret:=A) m v) ρ)).
 
-Definition TIdle {E VE F} (i : ThreadName) : @Prec E VE F :=
+Arguments SafeProg {E F VE VF} i impl R G {A} Q C Q0.
+
+Definition VerifyProg {E F VE VF A} i (impl : Impl E F)
+  (R G : @Relt E F VE VF)
+  (P : Prec VE VF)
+  (C : Prog E A)
+  (Q : Post VE VF A)
+  : Prop :=
+  SafeProg i impl R G (prComp P R) C Q.
+
+Definition TIdle {E F VE VF} (i : ThreadName) : @Prec E F VE VF :=
   fun s ρ =>
     fst s i = Idle /\
-    TraceIdle i ρ.
+    True. (* TODO: TraceIdle? *)
 
-Definition TInvoke {E VE F} impl (i : ThreadName) Ret (m : F Ret) : Relt E VE F :=
+Definition TInvoke {E F VE VF} impl (i : ThreadName) Ret (m : F Ret) : @Relt E F VE VF :=
   fun s ρ t σ =>
     TIdle i s ρ /\
-    σ = app ρ (cons (i, CallEv m) nil) /\
-    InterStep (impl:=impl) i s (i, OCallEv m) t.
+    InterStep (impl:=impl) i s (i, OCallEv m) t /\
+    σ.(PState) = ρ.(PState) /\
+    σ.(PCalls) = updThs ρ.(PCalls) i (Some (existT _ _ m)) /\
+    σ.(PRets) = ρ.(PRets).
 
-Definition InvokeAny {E VE F} impl i : Relt E VE F :=
+Definition InvokeAny {E F VE VF} impl i : @Relt E F VE VF :=
   fun s ρ t σ =>
     exists Ret (m : F Ret), TInvoke impl i Ret m s ρ t σ.
 
-Definition Returned {E VE F} (i : ThreadName) {Ret} (m : F Ret) : Relt E VE F :=
-  fun s ρ t σ =>
-    s = t /\
-    ρ = σ /\
+Definition Returned {E F VE VF} (i : ThreadName) {Ret} (m : F Ret) : @Prec E F VE VF :=
+  fun t σ =>
     exists (v : Ret), 
       fst t i = Cont m (Return v) /\
-      exists r,
-        projAgent i σ = app r (cons (i, RetEv m v) nil).
+      exists ρ,
+        σ.(PState) = ρ.(PState) /\
+        σ.(PCalls) = ρ.(PCalls) /\
+        updThs σ.(PRets) i (Some (existT _ _ v)) = ρ.(PRets).
 
-Definition TReturn {E VE F} (impl : Impl E F) (i : ThreadName) {Ret} (m : F Ret) : Relt E VE F :=
+Definition TReturn {E F VE VF} (impl : Impl E F) (i : ThreadName) {Ret} (m : F Ret) : @Relt E F VE VF :=
   fun s ρ t σ =>
     fst t i = Idle /\
     σ = ρ /\
-    exists (v : Ret) r,
-      projAgent i σ = app r (cons (i, RetEv m v) nil) /\
-      InterStep (impl:=impl) i s (i, ORetEv m v) t.
+    exists (v : Ret),
+      σ.(PState) = ρ.(PState) ->
+      σ.(PCalls) = ρ.(PCalls) ->
+      updThs σ.(PRets) i (Some (existT _ _ v)) = ρ.(PRets).
 
-Definition ReturnAny {E VE F} impl i : Relt E VE F :=
+Definition ReturnAny {E F VE VF} impl i : @Relt E F VE VF :=
   fun s ρ t σ =>
     exists Ret (m : F Ret), TReturn impl i m s ρ t σ.
+
+Definition initPoss {F VF} : @Poss F VF := {|
+  PState := VF.(Init);
+  PCalls _ := None;
+  PRets _ := None;
+|}.
 
 Definition VerifyImpl
   {E F}
   (VE : Spec E)
   (VF : Spec F)
-  (R G : ThreadName -> Relt E VE F)
-  (P : ThreadName -> forall Ret, F Ret -> @Prec E VE F)
+  (R G : ThreadName -> Relt VE VF)
+  (P : ThreadName -> forall Ret, F Ret -> Prec VE VF)
   (impl : Impl E F)
-  (Q : ThreadName -> forall Ret, F Ret -> Post E VE F Ret) : Prop :=
+  (Q : ThreadName -> forall Ret, F Ret -> Post VE VF Ret) : Prop :=
   (* Side conditions *)
   (forall i j, i <> j -> G i ==> R j) /\
   (forall i Ret (m : F Ret) v,
-    P i Ret m (allIdle, VE.(Init)) nil /\
+    P i Ret m (allIdle, VE.(Init)) initPoss /\
     P i Ret m ==> TIdle i /\
     Stable (R i) (P i Ret m) /\
     Stable (R i) (Q i Ret m v)) /\
   (forall i Ret1 (m1 : F Ret1) Ret2 (m2 : F Ret2) v,
-    P i Ret1 m1 <<- TInvoke impl i Ret1 m1 <<- Q i Ret1 m1 v <<- Returned i m1 <<- TReturn impl i m1 ==> P i Ret2 m2) /\
+    P i Ret1 m1 <<- TInvoke impl i Ret1 m1 <<- Q i Ret1 m1 v <<- PrecToRelt (Returned i m1) <<- TReturn impl i m1 ==> P i Ret2 m2) /\
   (* Verification task *)
   (forall i Ret (m : F Ret),
-    VerifyProg VF i impl (R i) (G i)
+    VerifyProg i impl (R i) (G i)
       (P i Ret m <<- TInvoke impl i Ret m)
       (impl Ret m)
-      (fun v s ρ t σ =>
-        Q i Ret m v s ρ t σ /\
-        Returned i m t σ t σ)).
+      (fun v => Q i Ret m v ->> PrecToRelt (Returned i m))).
