Core/Program.v
@@ -11,14 +11,12 @@ CoInductive Prog {E : ESig} {Ret : Type} : Type :=
 
 Arguments Prog : clear implicits.
 
-Notation "x <- f ; m" := (Bind f (fun x => m)) (at level 80, right associativity).
-
 Definition Impl {E : ESig} {F : ESig} := (forall Ret, F Ret -> Prog E Ret).
 Arguments Impl : clear implicits.
 
 (* Identity Program and Implementation *)
 Definition idProg {E : ESig} {Ret : Type} : E Ret -> Prog E Ret := 
-    fun e => (x <- e ; Return x).
+    fun e => (Bind e Return).
 
 Definition idImpl {E : ESig} : Impl E E := 
     fun Ret => idProg.
@@ -27,7 +25,7 @@ Definition idImpl {E : ESig} : Impl E E :=
 
 CoFixpoint bindProg {E A B} (p : Prog E A) (f : A -> Prog E B) : Prog E B :=
   match p with
-    | Bind e f' => x <- e; bindProg (f' x) f
+    | Bind e f' => Bind e (fun x => bindProg (f' x) f)
     | Return a => f a
     | NoOp p' => NoOp (bindProg p' f)
   end.
@@ -40,7 +38,7 @@ CoFixpoint mapProg
            (p : Prog E Ret) :
   Prog E' Ret :=
   match p with
-    | @Bind _ _ A e f' => a <- f A e; mapProg f (f' a)
+    | @Bind _ _ A e f' => Bind (f A e) (fun a => mapProg f (f' a))
     | Return r => Return r
     | NoOp p' => NoOp (mapProg f p')
   end.
@@ -61,7 +59,7 @@ with bindSubstProg
            {F F'} (impl : forall A, F' A -> Prog F A)
            {R R'} (f: R -> Prog F' R') (p: Prog F R) :=
   match p with
-  | Bind m' f' => r <- m'; bindSubstProg impl f (f' r)
+  | Bind m' f' => Bind m' (fun r => bindSubstProg impl f (f' r))
   | Return a => NoOp (substProg impl (f a))
   | NoOp p'' => NoOp (bindSubstProg impl f p'')
   end.
