Core/Syntax.v
@@ -1,0 +1,23 @@
+From LHL Require Import
+  Program.
+
+Section syntax.
+
+Context {E : ESig}.
+
+Definition ret {A} (v : A) : Prog E A :=
+  Return v.
+
+CoFixpoint bind {A B} (C : Prog E A) (k : A -> Prog E B) :=
+  match C with
+  | Bind m k' => Bind m (fun v => bind (k' v) k)
+  | Return v => k v
+  | NoOp C => NoOp (bind C k)
+  end.
+
+Definition call {A} (m : E A) : Prog E A :=
+  Bind m Return.
+
+End syntax.
+
+Notation "x <- f ; m" := (bind f (fun x => m)) (at level 80, right associativity).
